add and use func! Notation

bedrock2/src/bedrock2/Syntax.v
@@ -51,15 +51,10 @@ Module cmd.
   | interact (binds : list String.string) (action : String.string) (args: list expr).
 End cmd. Notation cmd := cmd.cmd.
 
-Definition func : Type := String.string * (list String.string * list String.string * cmd).
-#[deprecated(note="Use bedrock2.Syntax.func instead.")]
-Notation function := func.
-#[deprecated(note="Use bedrock2.Syntax.func instead.")]
-Notation bedrock_func := func.
+Definition func : Type := (list String.string * list String.string * cmd).
 
 Module Coercions.
   Import String.
   Coercion expr.var : string >-> expr.
   Coercion expr.literal : Z >-> expr.
-  Coercion name_of_func (f : func) := fst f.
 End Coercions.
