bedrock2/src/bedrock2Examples/swap.v
@@ -1,24 +1,18 @@
-Require Import bedrock2.NotationsCustomEntry.
+Require Import bedrock2.NotationsCustomEntry coqutil.Macros.WithBaseName.
 
 Import Syntax BinInt String List.ListNotations.
 Local Open Scope string_scope. Local Open Scope Z_scope. Local Open Scope list_scope.
 
-Definition swap : func :=
-  ("swap", (["a"; "b"], [], bedrock_func_body:(
+Definition swap := func! (a, b) {
   t = load(b);
   store(b, load(a));
   store(a, t)
-))).
+}.
 
-Definition swap_swap : func :=
-  ("swap_swap", (["a";"b"], [], bedrock_func_body:(
+Definition swap_swap := func! (a, b) {
   swap(a, b);
   swap(a, b)
-))).
-
-Definition main : func :=
-  ("main", ([], [], bedrock_func_body:(
-    swap_swap($100, $108)))).
+}.
 
 Require bedrock2.WeakestPrecondition.
 Require Import bedrock2.Semantics bedrock2.FE310CSemantics.
@@ -58,12 +52,12 @@ Section WithParameters.
     repeat (straightline || (straightline_call; [solve[SeparationLogic.ecancel_assumption]|])); []; eauto.
   Defined.
 
-  Lemma link_swap_swap_swap_swap : spec_of_swap_swap (swap_swap::swap::nil).
+  Lemma link_swap_swap_swap_swap : spec_of_swap_swap &[,swap_swap; swap].
   Proof. auto using swap_swap_ok, swap_ok. Qed.
 
   (* Print Assumptions link_swap_swap_swap_swap. *)
   (*
   From bedrock2 Require Import ToCString PrintString.
-  Goal True. print_string (c_module (swap_swap::swap::nil)). Abort.
+  Goal True. print_string (c_module &[,swap_swap; swap]). Abort.
   *)
 End WithParameters.
