compiler/src/compilerExamples/SpillingTests.v
@@ -3,36 +3,13 @@ Require Import bedrock2.NotationsCustomEntry.
 Import Syntax BinInt String List.ListNotations.
 Local Open Scope string_scope. Local Open Scope Z_scope. Local Open Scope list_scope.
 
-Definition swap : func := let a := "a" in let b := "b" in let t := "t" in
-  ("swap", ([a; b], [], bedrock_func_body:(
+Definition swap := func! (a, b) {
   t = load(b);
   store(b, load(a));
   store(a, t)
-))).
+}.
 
-Definition long1 : func :=
-  let a0 := "a0" in let b0 := "b0" in
-  let a1 := "a1" in let b1 := "b1" in
-  let a2 := "a2" in let b2 := "b2" in
-  let a3 := "a3" in let b3 := "b3" in
-  let a4 := "a4" in let b4 := "b4" in
-  let a5 := "a5" in let b5 := "b5" in
-  let a6 := "a6" in let b6 := "b6" in
-  let a7 := "a7" in let b7 := "b7" in
-  let a8 := "a8" in let b8 := "b8" in
-  let a9 := "a9" in let b9 := "b9" in
-  let a10 := "a10" in let b10 := "b10" in
-  let a11 := "a11" in let b11 := "b11" in
-  let a12 := "a12" in let b12 := "b12" in
-  let a13 := "a13" in let b13 := "b13" in
-  let a14 := "a14" in let b14 := "b14" in
-  let a15 := "a15" in let b15 := "b15" in
-  let a16 := "a16" in let b16 := "b16" in
-  let a17 := "a17" in let b17 := "b17" in
-  let a18 := "a18" in let b18 := "b18" in
-  let a19 := "a19" in let b19 := "b19" in
-  ("long1", ([a0; b0], [a19;b19], bedrock_func_body:(
-
+Definition long1 := func! (a0, b0) ~> (a19, b19) {
   (* TODO once spilling is improved, test that it still works if these two lines are removed
      (currently the test that all resnames are <32 fails if these two lines are removed) *)
   a19 = $0;
@@ -135,4 +112,4 @@ Definition long1 : func :=
 
   a19 = b0;
   b19 = b0
-))).
+}.
