bedrock2/src/bedrock2/PrintListByte.v
@@ -1,73 +1,11 @@
-Require Import Ltac2.Ltac2 Ltac2.Printf Coq.Strings.Ascii.
-(* Usage: see etc/bytedump.py and its invocation in bedrock2/Makefile *)
+Require Import coqutil.Tactics.ident_of_string Coq.Strings.String.
+From Ltac2 Require Import Ltac2 Printf Option Ltac1.
 
-Module Unsafe.
-  (* 0.6s/10k *)
-  Ltac2 char_of_constr_byte (b : constr) :=
-    let t := constr:(true) in
-    match Constr.Unsafe.kind (eval cbv in (ascii_of_byte $b)) with
-    | Constr.Unsafe.App _ args => Char.of_int
-      (Int.add (match Constr.equal (Array.get args 0) t with true => 1 | false => 0 end) (Int.mul 2 (
-      (Int.add (match Constr.equal (Array.get args 1) t with true => 1 | false => 0 end) (Int.mul 2 (
-      (Int.add (match Constr.equal (Array.get args 2) t with true => 1 | false => 0 end) (Int.mul 2 (
-      (Int.add (match Constr.equal (Array.get args 3) t with true => 1 | false => 0 end) (Int.mul 2 (
-      (Int.add (match Constr.equal (Array.get args 4) t with true => 1 | false => 0 end) (Int.mul 2 (
-      (Int.add (match Constr.equal (Array.get args 5) t with true => 1 | false => 0 end) (Int.mul 2 (
-      (Int.add (match Constr.equal (Array.get args 6) t with true => 1 | false => 0 end) (Int.mul 2 (
-      (Int.add (match Constr.equal (Array.get args 7) t with true => 1 | false => 0 end) 0))))))))))))))))))))))
-    | _ => Control.throw No_value
-    end.
-  
-  (* 1.2s/10k:
-  Ltac2 char_of_constr_byte (b : constr) :=
-    match Constr.Unsafe.kind constr:(Byte.byte) with
-    | Constr.Unsafe.Ind byte byteinstance =>
-      let rec f i :=
-        match Constr.equal b (Constr.Unsafe.make (Constr.Unsafe.Constructor (Constr.Unsafe.constructor byte i) byteinstance)) with
-        | true => i
-        | _ => f (Int.add 1 i)
-        end in Char.of_int (f 0)
-    | _ => Char.of_int 0
-    end .
-  *)
-  
-  Ltac2 rec length_constr_list (xs : constr) : int :=
-    match Constr.Unsafe.kind xs with
-    | Constr.Unsafe.App _ args =>
-      match Int.equal (Array.length args) 3 with
-      | true => Int.add 1 (length_constr_list (Array.get args 2))
-      | _ => 0
-      end
-    | Constr.Unsafe.Constructor _ _ => 0
-    | _ => Control.throw No_value
-    end.
-  
-  Ltac2 string_of_constr_list_byte (bs : constr) :=
-    let buf := String.make (length_constr_list bs) (Char.of_int 0) in
-    let rec fill (i : int)(bs : constr) :=
-      match Constr.Unsafe.kind bs with
-      | Constr.Unsafe.App _ args =>
-        match Int.equal (Array.length args) 3 with
-        | true =>
-            String.set buf i (char_of_constr_byte (Array.get args 1));
-            fill  (Int.add i 1) (Array.get args 2)
-        | false => ()
-        end
-      | _ => Control.throw No_value
-      end in
-    fill 0 bs; buf.
-End Unsafe.
-
-Ltac2 string_of_constr_list_byte (bs : constr) :=
-  let bs := eval vm_compute in ($bs : list Byte.byte) in
-  Unsafe.string_of_constr_list_byte bs.
-
-Ltac2 print_list_byte (bs : constr) := printf "%s" (string_of_constr_list_byte bs).
+Ltac2 print_list_byte (bs : constr) := printf "%s" (string_of_constr_string constr:(string_of_list_byte $bs)).
 Ltac print_list_byte := ltac2:(bs |- print_list_byte (Option.get (Ltac1.to_constr bs))).
 
 Ltac2 Notation "print_bytes" bs(constr) := print_list_byte bs.
 Tactic Notation "print_bytes" constr(bs) := print_list_byte bs.
-
 
 Require Import Coq.Lists.List.
 Definition allBytes: list Byte.byte :=
@@ -80,6 +18,6 @@ Definition allBytes: list Byte.byte :=
 (*
 Import ListNotations.
 Goal True.
-  Time print_bytes ([Byte.x41] ++ List.repeat Byte.x20 10000 ++ [Byte.x41]).
+  Time print_bytes ([Byte.x41] ++ List.repeat Byte.x20 10000 ++ [Byte.x41]). (*0.5s*)
 Abort.
 *)
