bedrock2/src/bedrock2Examples/uint128_32.v
@@ -3,8 +3,7 @@ Require Import bedrock2.NotationsCustomEntry.
 Import Syntax BinInt String List.ListNotations.
 Local Open Scope string_scope. Local Open Scope Z_scope. Local Open Scope list_scope.
 
-Definition uint128_add : func :=
-  ("uint128_add", (["s"; "a"; "b"], ["c"], bedrock_func_body:(
+Definition uint128_add := func! (s, a, b) ~> c {
   a0 = load4(a); a = a+$4;
   b0 = load4(b); b = b+$4;
   a1 = load4(a); a = a+$4;
@@ -38,7 +37,7 @@ Definition uint128_add : func :=
   c4p = s3 < c3;
   c = c + c4p;
   store4(s, s3)
-))).
+}.
 
 Require Import bedrock2.FE310CSemantics bedrock2.Semantics .
 Require Import bedrock2.WeakestPrecondition bedrock2.ProgramLogic.
